Foundation/Modal/Maximal/Basic.lean
@@ -6,7 +6,7 @@ namespace LO.Modal
 
 open LO.Entailment LO.Entailment.FiniteContext LO.Modal.Entailment
 
-variable {α} [DecidableEq α]
+variable {α} {φ ψ : Modal.Formula α}
 
 namespace Formula
 
@@ -19,8 +19,7 @@ postfix:75 "ᵀ" => trivTranslate
 
 namespace trivTranslate
 
-@[simp]
-lemma degree_zero : φᵀ.degree = 0 := by induction φ <;> simp [trivTranslate, degree, *];
+@[simp, grind! .] lemma degree_zero : φᵀ.degree = 0 := by induction φ <;> simp [trivTranslate, degree, *];
 
 @[simp]
 lemma toIP : φᵀ.toPropFormula = φᵀ := by
@@ -41,10 +40,10 @@ postfix:75 "ⱽ" => verTranslate
 
 namespace verTranslate
 
-@[simp]
+@[simp, grind .]
 lemma degree_zero : φⱽ.degree = 0 := by
   induction φ using rec' with
-  | himp => simp [verTranslate, *];
+  | himp => simp [degree, verTranslate, *];
   | _ => rfl;
 
 @[simp]
