Foundation/Modal/Neighborhood/AxiomGeach.lean
@@ -228,21 +228,21 @@ instance [Entailment.HasAxiomT 𝓢] : (basicCanonicity 𝓢).toModel.IsReflexiv
   apply Canonicity.isReflexive;
   intro X hX A hA;
   obtain ⟨φ, rfl, hφ⟩ := basicCanonicity.iff_mem_box_exists_fml.mp hA;
-  apply proofset.imp_subset.mp (by simp) hφ;
+  apply proofset.imp_subset.mp axiomT! hφ;
 
 instance [Entailment.HasAxiomFour 𝓢] : (basicCanonicity 𝓢).toModel.IsTransitive := by
   apply Canonicity.isTransitive;
   intro X hX A hA;
   obtain ⟨φ, rfl, hφ⟩ := basicCanonicity.iff_mem_box_exists_fml.mp hA;
   simp only [Canonicity.boxItr_proofset];
-  apply proofset.imp_subset.mp (by simp) hφ;
+  apply proofset.imp_subset.mp axiomFour! hφ;
 
 instance [Entailment.HasAxiomD 𝓢] : (basicCanonicity 𝓢).toModel.IsSerial := by
   apply Canonicity.isSerial;
   intro X hX A hA;
   obtain ⟨φ, rfl, hφ⟩ := basicCanonicity.iff_mem_box_exists_fml.mp hA;
   simp only [Canonicity.dia_proofset];
-  apply proofset.imp_subset.mp (by simp) hφ;
+  apply proofset.imp_subset.mp axiomD! hφ;
 
 
 namespace relativeBasicCanonicity
